src/specs/VerifyHighEncapsulatedToHigh.ec
@@ -35,6 +35,1481 @@ lemma verify_high_encapsulated_equiv_high:
     ].
     proof.
       proc.
+      seq 5 29: (
+        (failed{1} /\ !isValid{2}) \/ (
+        !failed{1} /\ isValid{2} /\
+        !vk_recursive_flag{1} /\
+        _public_input{1} = public_input{2} /\
+        _state_poly_0{1} = a{2} /\
+        _state_poly_1{1} = b{2} /\
+        _state_poly_2{1} = c{2} /\
+        _state_poly_3{1} = d{2} /\
+        _copy_permutation_grand_product{1} = z_perm{2} /\
+        _lookup_s_poly{1} = s{2} /\
+        _lookup_grand_product{1} = z_lookup{2} /\
+        _quotient_poly_part_0{1} = t_0{2} /\
+        _quotient_poly_part_1{1} = t_1{2} /\
+        _quotient_poly_part_2{1} = t_2{2} /\
+        _quotient_poly_part_3{1} = t_3{2} /\
+        _state_poly_0_opening_at_z{1} = a_at_z{2} /\
+        _state_poly_1_opening_at_z{1} = b_at_z{2} /\
+        _state_poly_2_opening_at_z{1} = c_at_z{2} /\
+        _state_poly_3_opening_at_z{1} = d_at_z{2} /\
+        _state_poly_3_opening_at_z_omega{1} = d_at_z_omega{2} /\
+        _gate_selector_0_opening_at_z{1} = main_gate_selector_at_z{2} /\
+        _copy_permutation_poly_0_opening_at_z{1} = sigma_0_at_z{2} /\
+        _copy_permutation_poly_1_opening_at_z{1} = sigma_1_at_z{2} /\ 
+        _copy_permutation_poly_2_opening_at_z{1} = sigma_2_at_z{2} /\
+        _copy_permutation_grand_product_opening_at_z_omega{1} = z_perm_at_z_omega{2} /\
+        _lookup_s_poly_opening_at_z_omega{1} = s_at_z_omega{2} /\
+        _lookup_grand_product_opening_at_z_omega{1} = z_lookup_at_z_omega{2} /\
+        _lookup_t_poly_opening_at_z{1} = t_at_z{2} /\
+        _lookup_t_poly_opening_at_z_omega{1} = t_at_z_omega{2} /\
+        _lookup_selector_poly_opening_at_z{1} = lookup_selector_at_z{2} /\
+        _lookup_table_type_poly_opening_at_z{1} = table_type_at_z{2} /\
+        _quotient_poly_opening_at_z{1} = quotient_poly_opening_at_z{2} /\
+        _linearisation_poly_opening_at_z{1} = r_at_z{2} /\
+        _opening_proof_at_z{1} = w{2} /\
+        _opening_proof_at_z_omega{1} = w'{2} /\
+        _recursive_part_p1{1} = None /\
+        _recursive_part_p2{1} = None /\
+        k0{2} = FieldR.inF Constants.NON_RESIDUE_0 /\
+        k1{2} = FieldR.inF Constants.NON_RESIDUE_1 /\ 
+        k2{2} = FieldR.inF Constants.NON_RESIDUE_2 /\
+        n{2} = Constants.DOMAIN_SIZE /\
+        q_a{2} = vk_gate_setup_0 /\
+        q_b{2} = vk_gate_setup_1 /\
+        q_c{2} = vk_gate_setup_2 /\
+        q_d{2} = vk_gate_setup_3 /\
+        q_ab{2} = vk_gate_setup_4 /\
+        q_ac{2} = vk_gate_setup_5 /\
+        q_const{2} = vk_gate_setup_6 /\
+        q_d_next{2} = vk_gate_setup_7 /\
+        custom_gate_selector{2} = vk_gate_selectors_1 /\
+        sigma_0{2} = vk_permutation_0 /\
+        sigma_1{2} = vk_permutation_1 /\
+        sigma_2{2} = vk_permutation_2 /\ 
+        sigma_3{2} = vk_permutation_3 /\
+        lookup_selector{2} = vk_lookup_selector /\
+        table_type{2} = vk_lookup_table_type /\
+        omega{2} = Constants.OMEGAFr /\
+        col_0{2} = vk_lookup_table_0 /\
+        col_1{2} = vk_lookup_table_1 /\
+        col_2{2} = vk_lookup_table_2 /\
+        col_3{2} = vk_lookup_table_3
+      )).
+        inline LoadProof.high.
+        rcondf{1} 43. progress. wp. skip. by progress.
+        case (
+          public_input_length_in_words{1} = 1 /\
+          proof_length_in_words{1} = 44 /\
+          recursive_proof_length_in_words{1} = 0
+        ).
+          rcondt{1} 46. progress. wp. skip. by progress.
+          wp. skip. by progress.
+        (* false case *)
+          rcondf{1} 46. progress. wp. skip. progress. rewrite -andbA. assumption.
+          wp. skip. progress. rewrite -andbA. assumption.
+
+      (* load proof done *)
+
+      (* initialize transcript *)
+      seq 1 16: (
+        (failed{1} /\ !isValid{2}) \/ (
+        !failed{1} /\ isValid{2} /\
+        !vk_recursive_flag{1} /\
+        _public_input{1} = public_input{2} /\
+        _state_poly_0{1} = a{2} /\
+        _state_poly_1{1} = b{2} /\
+        _state_poly_2{1} = c{2} /\
+        _state_poly_3{1} = d{2} /\
+        _copy_permutation_grand_product{1} = z_perm{2} /\
+        _lookup_s_poly{1} = s{2} /\
+        _lookup_grand_product{1} = z_lookup{2} /\
+        _quotient_poly_part_0{1} = t_0{2} /\
+        _quotient_poly_part_1{1} = t_1{2} /\
+        _quotient_poly_part_2{1} = t_2{2} /\
+        _quotient_poly_part_3{1} = t_3{2} /\
+        _state_poly_0_opening_at_z{1} = a_at_z{2} /\
+        _state_poly_1_opening_at_z{1} = b_at_z{2} /\
+        _state_poly_2_opening_at_z{1} = c_at_z{2} /\
+        _state_poly_3_opening_at_z{1} = d_at_z{2} /\
+        _state_poly_3_opening_at_z_omega{1} = d_at_z_omega{2} /\
+        _gate_selector_0_opening_at_z{1} = main_gate_selector_at_z{2} /\
+        _copy_permutation_poly_0_opening_at_z{1} = sigma_0_at_z{2} /\
+        _copy_permutation_poly_1_opening_at_z{1} = sigma_1_at_z{2} /\ 
+        _copy_permutation_poly_2_opening_at_z{1} = sigma_2_at_z{2} /\
+        _copy_permutation_grand_product_opening_at_z_omega{1} = z_perm_at_z_omega{2} /\
+        _lookup_s_poly_opening_at_z_omega{1} = s_at_z_omega{2} /\
+        _lookup_grand_product_opening_at_z_omega{1} = z_lookup_at_z_omega{2} /\
+        _lookup_t_poly_opening_at_z{1} = t_at_z{2} /\
+        _lookup_t_poly_opening_at_z_omega{1} = t_at_z_omega{2} /\
+        _lookup_selector_poly_opening_at_z{1} = lookup_selector_at_z{2} /\
+        _lookup_table_type_poly_opening_at_z{1} = table_type_at_z{2} /\
+        _quotient_poly_opening_at_z{1} = quotient_poly_opening_at_z{2} /\
+        _linearisation_poly_opening_at_z{1} = r_at_z{2} /\
+        _opening_proof_at_z{1} = w{2} /\
+        _opening_proof_at_z_omega{1} = w'{2} /\
+        _recursive_part_p1{1} = None /\
+        _recursive_part_p2{1} = None /\
+        k0{2} = FieldR.inF Constants.NON_RESIDUE_0 /\
+        k1{2} = FieldR.inF Constants.NON_RESIDUE_1 /\ 
+        k2{2} = FieldR.inF Constants.NON_RESIDUE_2 /\
+        n{2} = Constants.DOMAIN_SIZE /\
+        q_a{2} = vk_gate_setup_0 /\
+        q_b{2} = vk_gate_setup_1 /\
+        q_c{2} = vk_gate_setup_2 /\
+        q_d{2} = vk_gate_setup_3 /\
+        q_ab{2} = vk_gate_setup_4 /\
+        q_ac{2} = vk_gate_setup_5 /\
+        q_const{2} = vk_gate_setup_6 /\
+        q_d_next{2} = vk_gate_setup_7 /\
+        custom_gate_selector{2} = vk_gate_selectors_1 /\
+        sigma_0{2} = vk_permutation_0 /\
+        sigma_1{2} = vk_permutation_1 /\
+        sigma_2{2} = vk_permutation_2 /\ 
+        sigma_3{2} = vk_permutation_3 /\
+        lookup_selector{2} = vk_lookup_selector /\
+        table_type{2} = vk_lookup_table_type /\
+        omega{2} = Constants.OMEGAFr /\
+        col_0{2} = vk_lookup_table_0 /\
+        col_1{2} = vk_lookup_table_1 /\
+        col_2{2} = vk_lookup_table_2 /\
+        col_3{2} = vk_lookup_table_3 /\
+        state_alpha{1} = alpha{2} /\
+        state_beta{1} = beta_{2} /\
+        state_beta_lookup{1} = beta'{2} /\
+        state_gamma{1} = gamma{2} /\
+        state_gamma_lookup{1} = gamma'{2} /\
+        state_eta{1} = eta_{2} /\
+        state_z{1} = z{2} /\
+        state_z_in_domain{1} = z{2} ^ n{2} /\
+        state_v{1} = v{2} /\
+        state_u{1} = u{2} 
+      )).
+        inline InitializeTranscript.high.
+        case (failed{1}).
+          conseq (_ : (failed{1} /\ !isValid{2}) ==> (failed{1} /\ !isValid{2})).
+            progress. by case H; progress.
+            progress. left. by progress.
+          wp. skip. by progress.
+        (* case !failed{1} *)
+          cfold{1} 1. cfold{1} 1.
+          sp 32 0.
+
+          conseq (_ : (
+            !failed{1} /\
+            isValid{2} /\
+            !vk_recursive_flag{1} /\
+            _public_input{1} = public_input{2} /\
+            _state_poly_0{1} = a{2} /\
+            _state_poly_1{1} = b{2} /\
+            _state_poly_2{1} = c{2} /\
+            _state_poly_3{1} = d{2} /\
+            _copy_permutation_grand_product{1} = z_perm{2} /\
+            _lookup_s_poly{1} = s{2} /\
+            _lookup_grand_product{1} = z_lookup{2} /\
+            _quotient_poly_part_0{1} = t_0{2} /\
+            _quotient_poly_part_1{1} = t_1{2} /\
+            _quotient_poly_part_2{1} = t_2{2} /\
+            _quotient_poly_part_3{1} = t_3{2} /\
+            _state_poly_0_opening_at_z{1} = a_at_z{2} /\
+            _state_poly_1_opening_at_z{1} = b_at_z{2} /\
+            _state_poly_2_opening_at_z{1} = c_at_z{2} /\
+            _state_poly_3_opening_at_z{1} = d_at_z{2} /\
+            _state_poly_3_opening_at_z_omega{1} = d_at_z_omega{2} /\
+            _gate_selector_0_opening_at_z{1} = main_gate_selector_at_z{2} /\
+            _copy_permutation_poly_0_opening_at_z{1} = sigma_0_at_z{2} /\
+            _copy_permutation_poly_1_opening_at_z{1} = sigma_1_at_z{2} /\
+            _copy_permutation_poly_2_opening_at_z{1} = sigma_2_at_z{2} /\
+            _copy_permutation_grand_product_opening_at_z_omega{1} = z_perm_at_z_omega{2} /\
+            _lookup_s_poly_opening_at_z_omega{1} = s_at_z_omega{2} /\
+            _lookup_grand_product_opening_at_z_omega{1} = z_lookup_at_z_omega{2} /\
+            _lookup_t_poly_opening_at_z{1} = t_at_z{2} /\
+            _lookup_t_poly_opening_at_z_omega{1} = t_at_z_omega{2} /\
+            _lookup_selector_poly_opening_at_z{1} = lookup_selector_at_z{2} /\
+            _lookup_table_type_poly_opening_at_z{1} = table_type_at_z{2} /\
+            _quotient_poly_opening_at_z{1} = quotient_poly_opening_at_z{2} /\
+            _linearisation_poly_opening_at_z{1} = r_at_z{2} /\
+            _opening_proof_at_z{1} = w{2} /\
+            _opening_proof_at_z_omega{1} = w'{2} /\
+            _recursive_part_p1{1} = None /\
+            _recursive_part_p2{1} = None /\
+            k0{2} = (FieldR.inF Constants.NON_RESIDUE_0) /\
+            k1{2} = (FieldR.inF Constants.NON_RESIDUE_1) /\
+            k2{2} = (FieldR.inF Constants.NON_RESIDUE_2) /\
+            n{2} = Constants.DOMAIN_SIZE /\
+            q_a{2} = vk_gate_setup_0 /\
+            q_b{2} = vk_gate_setup_1 /\
+            q_c{2} = vk_gate_setup_2 /\
+            q_d{2} = vk_gate_setup_3 /\
+            q_ab{2} = vk_gate_setup_4 /\
+            q_ac{2} = vk_gate_setup_5 /\
+            q_const{2} = vk_gate_setup_6 /\
+            q_d_next{2} = vk_gate_setup_7 /\
+            custom_gate_selector{2} = vk_gate_selectors_1 /\
+            sigma_0{2} = vk_permutation_0 /\
+            sigma_1{2} = vk_permutation_1 /\
+            sigma_2{2} = vk_permutation_2 /\
+            sigma_3{2} = vk_permutation_3 /\
+            lookup_selector{2} = vk_lookup_selector /\
+            table_type{2} = vk_lookup_table_type /\
+            omega{2} = Constants.OMEGAFr /\
+            col_0{2} = vk_lookup_table_0 /\
+            col_1{2} = vk_lookup_table_1 /\
+            col_2{2} = vk_lookup_table_2 /\
+            col_3{2} = vk_lookup_table_3 /\
+            n{2} = Constants.DOMAIN_SIZE /\
+            proofOpeningProofAtZ{1} = w{2} /\
+            proofOpeningProofAtZOmega{1} = w'{2} /\
+            proofQuotientPolyOpeningAtZ{1} = quotient_poly_opening_at_z{2} /\
+            proofStatePolys0OpeningAtZ{1} = a_at_z{2} /\
+            proofStatePolys1OpeningAtZ{1} = b_at_z{2} /\
+            proofStatePolys2OpeningAtZ{1} = c_at_z{2} /\
+            proofStatePolys3OpeningAtZ{1} = d_at_z{2} /\
+            proofStatePolys3OpeningAtZOmega{1} = d_at_z_omega{2} /\
+            proofGateSelectors0OpeningAtZ{1} = main_gate_selector_at_z{2} /\
+            proofCopyPermutationPolys0OpeningAtZ{1} = sigma_0_at_z{2} /\
+            proofCopyPermutationPolys1OpeningAtZ{1} = sigma_1_at_z{2} /\
+            proofCopyPermutationPolys2OpeningAtZ{1} = sigma_2_at_z{2} /\
+            proofCopyPermutationGrandProductOpeningAtZOmega{1} = z_perm_at_z_omega{2} /\
+            proofLookupTPolyOpeningAtZ{1} = t_at_z{2} /\
+            proofLookupSelectorPolyOpeningAtZ{1} = lookup_selector_at_z{2} /\
+            proofLookupTableTypePolyOpeningAtZ{1} = table_type_at_z{2} /\
+            proofLookupSPolyOpeningAtZOmega{1} = s_at_z_omega{2} /\
+            proofLookupGrandProductOpeningAtZOmega{1} = z_lookup_at_z_omega{2} /\
+            proofLookupTPolyOpeningAtZOmega{1} = t_at_z_omega{2} /\
+            proofLinearisationPolyOpeningAtZ{1} = r_at_z{2} /\
+            publicInput{1} = public_input{2} /\
+            proofStatePolys0{1} = a{2} /\
+            proofStatePolys1{1} = b{2} /\
+            proofStatePolys2{1} = c{2} /\
+            proofStatePolys3{1} = d{2} /\
+            proofLookupSPoly{1} = s{2} /\
+            proofCopyPermutationGrandProduct{1} = z_perm{2} /\
+            proofLookupGrandProduct{1} = z_lookup{2} /\
+            proofQuotientPolyParts0{1} = t_0{2} /\
+            proofQuotientPolyParts1{1} = t_1{2} /\
+            proofQuotientPolyParts2{1} = t_2{2} /\
+            proofQuotientPolyParts3{1} = t_3{2}
+          ) ==> _). by progress; case H; progress.
+            
+          seq 19 2: (
+            #pre /\
+            state{2} = (state0_8{1}, state1_8{1}) /\
+            stateEta{1} = eta_{2}          
+          ).
+            wp. skip. rewrite /commit_fr /commit_g. by progress.
+
+          seq 6 3: (
+            !failed{1} /\
+            isValid{2} /\
+            !vk_recursive_flag{1} /\
+            _public_input{1} = public_input{2} /\
+            _state_poly_0{1} = a{2} /\
+            _state_poly_1{1} = b{2} /\
+            _state_poly_2{1} = c{2} /\
+            _state_poly_3{1} = d{2} /\
+            _copy_permutation_grand_product{1} = z_perm{2} /\
+            _lookup_s_poly{1} = s{2} /\
+            _lookup_grand_product{1} = z_lookup{2} /\
+            _quotient_poly_part_0{1} = t_0{2} /\
+            _quotient_poly_part_1{1} = t_1{2} /\
+            _quotient_poly_part_2{1} = t_2{2} /\
+            _quotient_poly_part_3{1} = t_3{2} /\
+            _state_poly_0_opening_at_z{1} = a_at_z{2} /\
+            _state_poly_1_opening_at_z{1} = b_at_z{2} /\
+            _state_poly_2_opening_at_z{1} = c_at_z{2} /\
+            _state_poly_3_opening_at_z{1} = d_at_z{2} /\
+            _state_poly_3_opening_at_z_omega{1} = d_at_z_omega{2} /\
+            _gate_selector_0_opening_at_z{1} = main_gate_selector_at_z{2} /\
+            _copy_permutation_poly_0_opening_at_z{1} = sigma_0_at_z{2} /\
+            _copy_permutation_poly_1_opening_at_z{1} = sigma_1_at_z{2} /\
+            _copy_permutation_poly_2_opening_at_z{1} = sigma_2_at_z{2} /\
+            _copy_permutation_grand_product_opening_at_z_omega{1} = z_perm_at_z_omega{2} /\
+            _lookup_s_poly_opening_at_z_omega{1} = s_at_z_omega{2} /\
+            _lookup_grand_product_opening_at_z_omega{1} = z_lookup_at_z_omega{2} /\
+            _lookup_t_poly_opening_at_z{1} = t_at_z{2} /\
+            _lookup_t_poly_opening_at_z_omega{1} = t_at_z_omega{2} /\
+            _lookup_selector_poly_opening_at_z{1} = lookup_selector_at_z{2} /\
+            _lookup_table_type_poly_opening_at_z{1} = table_type_at_z{2} /\
+            _quotient_poly_opening_at_z{1} = quotient_poly_opening_at_z{2} /\
+            _linearisation_poly_opening_at_z{1} = r_at_z{2} /\
+            _opening_proof_at_z{1} = w{2} /\
+            _opening_proof_at_z_omega{1} = w'{2} /\
+            _recursive_part_p1{1} = None /\
+            _recursive_part_p2{1} = None /\
+            k0{2} = (FieldR.inF Constants.NON_RESIDUE_0) /\
+            k1{2} = (FieldR.inF Constants.NON_RESIDUE_1) /\
+            k2{2} = (FieldR.inF Constants.NON_RESIDUE_2) /\
+            n{2} = Constants.DOMAIN_SIZE /\
+            q_a{2} = vk_gate_setup_0 /\
+            q_b{2} = vk_gate_setup_1 /\
+            q_c{2} = vk_gate_setup_2 /\
+            q_d{2} = vk_gate_setup_3 /\
+            q_ab{2} = vk_gate_setup_4 /\
+            q_ac{2} = vk_gate_setup_5 /\
+            q_const{2} = vk_gate_setup_6 /\
+            q_d_next{2} = vk_gate_setup_7 /\
+            custom_gate_selector{2} = vk_gate_selectors_1 /\
+            sigma_0{2} = vk_permutation_0 /\
+            sigma_1{2} = vk_permutation_1 /\
+            sigma_2{2} = vk_permutation_2 /\
+            sigma_3{2} = vk_permutation_3 /\
+            lookup_selector{2} = vk_lookup_selector /\
+            table_type{2} = vk_lookup_table_type /\
+            omega{2} = Constants.OMEGAFr /\
+            col_0{2} = vk_lookup_table_0 /\
+            col_1{2} = vk_lookup_table_1 /\
+            col_2{2} = vk_lookup_table_2 /\
+            col_3{2} = vk_lookup_table_3 /\
+            n{2} = Constants.DOMAIN_SIZE /\
+            proofOpeningProofAtZ{1} = w{2} /\
+            proofOpeningProofAtZOmega{1} = w'{2} /\
+            proofQuotientPolyOpeningAtZ{1} = quotient_poly_opening_at_z{2} /\
+            proofStatePolys0OpeningAtZ{1} = a_at_z{2} /\
+            proofStatePolys1OpeningAtZ{1} = b_at_z{2} /\
+            proofStatePolys2OpeningAtZ{1} = c_at_z{2} /\
+            proofStatePolys3OpeningAtZ{1} = d_at_z{2} /\
+            proofStatePolys3OpeningAtZOmega{1} = d_at_z_omega{2} /\
+            proofGateSelectors0OpeningAtZ{1} = main_gate_selector_at_z{2} /\
+            proofCopyPermutationPolys0OpeningAtZ{1} = sigma_0_at_z{2} /\
+            proofCopyPermutationPolys1OpeningAtZ{1} = sigma_1_at_z{2} /\
+            proofCopyPermutationPolys2OpeningAtZ{1} = sigma_2_at_z{2} /\
+            proofCopyPermutationGrandProductOpeningAtZOmega{1} = z_perm_at_z_omega{2} /\
+            proofLookupTPolyOpeningAtZ{1} = t_at_z{2} /\
+            proofLookupSelectorPolyOpeningAtZ{1} = lookup_selector_at_z{2} /\
+            proofLookupTableTypePolyOpeningAtZ{1} = table_type_at_z{2} /\
+            proofLookupSPolyOpeningAtZOmega{1} = s_at_z_omega{2} /\
+            proofLookupGrandProductOpeningAtZOmega{1} = z_lookup_at_z_omega{2} /\
+            proofLookupTPolyOpeningAtZOmega{1} = t_at_z_omega{2} /\
+            proofLinearisationPolyOpeningAtZ{1} = r_at_z{2} /\
+            proofCopyPermutationGrandProduct{1} = z_perm{2} /\
+            proofLookupGrandProduct{1} = z_lookup{2} /\
+            proofQuotientPolyParts0{1} = t_0{2} /\
+            proofQuotientPolyParts1{1} = t_1{2} /\
+            proofQuotientPolyParts2{1} = t_2{2} /\
+            proofQuotientPolyParts3{1} = t_3{2} /\
+            state{2} = (state0_10{1}, state1_10{1}) /\
+            stateBeta{1} = beta_{2} /\
+            stateGamma{1} = gamma{2} /\
+            stateEta{1} = eta_{2}
+          ).
+            wp. skip. rewrite /commit_fr /commit_g. by progress.
+
+          seq 6 3: (
+            !failed{1} /\
+            isValid{2} /\
+            !vk_recursive_flag{1} /\
+            _public_input{1} = public_input{2} /\
+            _state_poly_0{1} = a{2} /\
+            _state_poly_1{1} = b{2} /\
+            _state_poly_2{1} = c{2} /\
+            _state_poly_3{1} = d{2} /\
+            _copy_permutation_grand_product{1} = z_perm{2} /\
+            _lookup_s_poly{1} = s{2} /\
+            _lookup_grand_product{1} = z_lookup{2} /\
+            _quotient_poly_part_0{1} = t_0{2} /\
+            _quotient_poly_part_1{1} = t_1{2} /\
+            _quotient_poly_part_2{1} = t_2{2} /\
+            _quotient_poly_part_3{1} = t_3{2} /\
+            _state_poly_0_opening_at_z{1} = a_at_z{2} /\
+            _state_poly_1_opening_at_z{1} = b_at_z{2} /\
+            _state_poly_2_opening_at_z{1} = c_at_z{2} /\
+            _state_poly_3_opening_at_z{1} = d_at_z{2} /\
+            _state_poly_3_opening_at_z_omega{1} = d_at_z_omega{2} /\
+            _gate_selector_0_opening_at_z{1} = main_gate_selector_at_z{2} /\
+            _copy_permutation_poly_0_opening_at_z{1} = sigma_0_at_z{2} /\
+            _copy_permutation_poly_1_opening_at_z{1} = sigma_1_at_z{2} /\
+            _copy_permutation_poly_2_opening_at_z{1} = sigma_2_at_z{2} /\
+            _copy_permutation_grand_product_opening_at_z_omega{1} = z_perm_at_z_omega{2} /\
+            _lookup_s_poly_opening_at_z_omega{1} = s_at_z_omega{2} /\
+            _lookup_grand_product_opening_at_z_omega{1} = z_lookup_at_z_omega{2} /\
+            _lookup_t_poly_opening_at_z{1} = t_at_z{2} /\
+            _lookup_t_poly_opening_at_z_omega{1} = t_at_z_omega{2} /\
+            _lookup_selector_poly_opening_at_z{1} = lookup_selector_at_z{2} /\
+            _lookup_table_type_poly_opening_at_z{1} = table_type_at_z{2} /\
+            _quotient_poly_opening_at_z{1} = quotient_poly_opening_at_z{2} /\
+            _linearisation_poly_opening_at_z{1} = r_at_z{2} /\
+            _opening_proof_at_z{1} = w{2} /\
+            _opening_proof_at_z_omega{1} = w'{2} /\
+            _recursive_part_p1{1} = None /\
+            _recursive_part_p2{1} = None /\
+            k0{2} = (FieldR.inF Constants.NON_RESIDUE_0) /\
+            k1{2} = (FieldR.inF Constants.NON_RESIDUE_1) /\
+            k2{2} = (FieldR.inF Constants.NON_RESIDUE_2) /\
+            n{2} = Constants.DOMAIN_SIZE /\
+            q_a{2} = vk_gate_setup_0 /\
+            q_b{2} = vk_gate_setup_1 /\
+            q_c{2} = vk_gate_setup_2 /\
+            q_d{2} = vk_gate_setup_3 /\
+            q_ab{2} = vk_gate_setup_4 /\
+            q_ac{2} = vk_gate_setup_5 /\
+            q_const{2} = vk_gate_setup_6 /\
+            q_d_next{2} = vk_gate_setup_7 /\
+            custom_gate_selector{2} = vk_gate_selectors_1 /\
+            sigma_0{2} = vk_permutation_0 /\
+            sigma_1{2} = vk_permutation_1 /\
+            sigma_2{2} = vk_permutation_2 /\
+            sigma_3{2} = vk_permutation_3 /\
+            lookup_selector{2} = vk_lookup_selector /\
+            table_type{2} = vk_lookup_table_type /\
+            omega{2} = Constants.OMEGAFr /\
+            col_0{2} = vk_lookup_table_0 /\
+            col_1{2} = vk_lookup_table_1 /\
+            col_2{2} = vk_lookup_table_2 /\
+            col_3{2} = vk_lookup_table_3 /\
+            n{2} = Constants.DOMAIN_SIZE /\
+            proofOpeningProofAtZ{1} = w{2} /\
+            proofOpeningProofAtZOmega{1} = w'{2} /\
+            proofQuotientPolyOpeningAtZ{1} = quotient_poly_opening_at_z{2} /\
+            proofStatePolys0OpeningAtZ{1} = a_at_z{2} /\
+            proofStatePolys1OpeningAtZ{1} = b_at_z{2} /\
+            proofStatePolys2OpeningAtZ{1} = c_at_z{2} /\
+            proofStatePolys3OpeningAtZ{1} = d_at_z{2} /\
+            proofStatePolys3OpeningAtZOmega{1} = d_at_z_omega{2} /\
+            proofGateSelectors0OpeningAtZ{1} = main_gate_selector_at_z{2} /\
+            proofCopyPermutationPolys0OpeningAtZ{1} = sigma_0_at_z{2} /\
+            proofCopyPermutationPolys1OpeningAtZ{1} = sigma_1_at_z{2} /\
+            proofCopyPermutationPolys2OpeningAtZ{1} = sigma_2_at_z{2} /\
+            proofCopyPermutationGrandProductOpeningAtZOmega{1} = z_perm_at_z_omega{2} /\
+            proofLookupTPolyOpeningAtZ{1} = t_at_z{2} /\
+            proofLookupSelectorPolyOpeningAtZ{1} = lookup_selector_at_z{2} /\
+            proofLookupTableTypePolyOpeningAtZ{1} = table_type_at_z{2} /\
+            proofLookupSPolyOpeningAtZOmega{1} = s_at_z_omega{2} /\
+            proofLookupGrandProductOpeningAtZOmega{1} = z_lookup_at_z_omega{2} /\
+            proofLookupTPolyOpeningAtZOmega{1} = t_at_z_omega{2} /\
+            proofLinearisationPolyOpeningAtZ{1} = r_at_z{2} /\
+            proofLookupGrandProduct{1} = z_lookup{2} /\
+            proofQuotientPolyParts0{1} = t_0{2} /\
+            proofQuotientPolyParts1{1} = t_1{2} /\
+            proofQuotientPolyParts2{1} = t_2{2} /\
+            proofQuotientPolyParts3{1} = t_3{2} /\
+            state{2} = (state0_12{1}, state1_12{1}) /\
+            stateBeta{1} = beta_{2} /\
+            stateGamma{1} = gamma{2} /\
+            stateBetaLookup{1} = beta'{2} /\
+            stateGammaLookup{1} = gamma'{2} /\
+            stateEta{1} = eta_{2}
+          ).
+            wp. skip. rewrite /commit_fr /commit_g. by progress.
+
+          seq 5 2: (
+            !failed{1} /\
+            isValid{2} /\
+            !vk_recursive_flag{1} /\
+            _public_input{1} = public_input{2} /\
+            _state_poly_0{1} = a{2} /\
+            _state_poly_1{1} = b{2} /\
+            _state_poly_2{1} = c{2} /\
+            _state_poly_3{1} = d{2} /\
+            _copy_permutation_grand_product{1} = z_perm{2} /\
+            _lookup_s_poly{1} = s{2} /\
+            _lookup_grand_product{1} = z_lookup{2} /\
+            _quotient_poly_part_0{1} = t_0{2} /\
+            _quotient_poly_part_1{1} = t_1{2} /\
+            _quotient_poly_part_2{1} = t_2{2} /\
+            _quotient_poly_part_3{1} = t_3{2} /\
+            _state_poly_0_opening_at_z{1} = a_at_z{2} /\
+            _state_poly_1_opening_at_z{1} = b_at_z{2} /\
+            _state_poly_2_opening_at_z{1} = c_at_z{2} /\
+            _state_poly_3_opening_at_z{1} = d_at_z{2} /\
+            _state_poly_3_opening_at_z_omega{1} = d_at_z_omega{2} /\
+            _gate_selector_0_opening_at_z{1} = main_gate_selector_at_z{2} /\
+            _copy_permutation_poly_0_opening_at_z{1} = sigma_0_at_z{2} /\
+            _copy_permutation_poly_1_opening_at_z{1} = sigma_1_at_z{2} /\
+            _copy_permutation_poly_2_opening_at_z{1} = sigma_2_at_z{2} /\
+            _copy_permutation_grand_product_opening_at_z_omega{1} = z_perm_at_z_omega{2} /\
+            _lookup_s_poly_opening_at_z_omega{1} = s_at_z_omega{2} /\
+            _lookup_grand_product_opening_at_z_omega{1} = z_lookup_at_z_omega{2} /\
+            _lookup_t_poly_opening_at_z{1} = t_at_z{2} /\
+            _lookup_t_poly_opening_at_z_omega{1} = t_at_z_omega{2} /\
+            _lookup_selector_poly_opening_at_z{1} = lookup_selector_at_z{2} /\
+            _lookup_table_type_poly_opening_at_z{1} = table_type_at_z{2} /\
+            _quotient_poly_opening_at_z{1} = quotient_poly_opening_at_z{2} /\
+            _linearisation_poly_opening_at_z{1} = r_at_z{2} /\
+            _opening_proof_at_z{1} = w{2} /\
+            _opening_proof_at_z_omega{1} = w'{2} /\
+            _recursive_part_p1{1} = None /\
+            _recursive_part_p2{1} = None /\
+            k0{2} = (FieldR.inF Constants.NON_RESIDUE_0) /\
+            k1{2} = (FieldR.inF Constants.NON_RESIDUE_1) /\
+            k2{2} = (FieldR.inF Constants.NON_RESIDUE_2) /\
+            n{2} = Constants.DOMAIN_SIZE /\
+            q_a{2} = vk_gate_setup_0 /\
+            q_b{2} = vk_gate_setup_1 /\
+            q_c{2} = vk_gate_setup_2 /\
+            q_d{2} = vk_gate_setup_3 /\
+            q_ab{2} = vk_gate_setup_4 /\
+            q_ac{2} = vk_gate_setup_5 /\
+            q_const{2} = vk_gate_setup_6 /\
+            q_d_next{2} = vk_gate_setup_7 /\
+            custom_gate_selector{2} = vk_gate_selectors_1 /\
+            sigma_0{2} = vk_permutation_0 /\
+            sigma_1{2} = vk_permutation_1 /\
+            sigma_2{2} = vk_permutation_2 /\
+            sigma_3{2} = vk_permutation_3 /\
+            lookup_selector{2} = vk_lookup_selector /\
+            table_type{2} = vk_lookup_table_type /\
+            omega{2} = Constants.OMEGAFr /\
+            col_0{2} = vk_lookup_table_0 /\
+            col_1{2} = vk_lookup_table_1 /\
+            col_2{2} = vk_lookup_table_2 /\
+            col_3{2} = vk_lookup_table_3 /\
+            n{2} = Constants.DOMAIN_SIZE /\
+            proofOpeningProofAtZ{1} = w{2} /\
+            proofOpeningProofAtZOmega{1} = w'{2} /\
+            proofQuotientPolyOpeningAtZ{1} = quotient_poly_opening_at_z{2} /\
+            proofStatePolys0OpeningAtZ{1} = a_at_z{2} /\
+            proofStatePolys1OpeningAtZ{1} = b_at_z{2} /\
+            proofStatePolys2OpeningAtZ{1} = c_at_z{2} /\
+            proofStatePolys3OpeningAtZ{1} = d_at_z{2} /\
+            proofStatePolys3OpeningAtZOmega{1} = d_at_z_omega{2} /\
+            proofGateSelectors0OpeningAtZ{1} = main_gate_selector_at_z{2} /\
+            proofCopyPermutationPolys0OpeningAtZ{1} = sigma_0_at_z{2} /\
+            proofCopyPermutationPolys1OpeningAtZ{1} = sigma_1_at_z{2} /\
+            proofCopyPermutationPolys2OpeningAtZ{1} = sigma_2_at_z{2} /\
+            proofCopyPermutationGrandProductOpeningAtZOmega{1} = z_perm_at_z_omega{2} /\
+            proofLookupTPolyOpeningAtZ{1} = t_at_z{2} /\
+            proofLookupSelectorPolyOpeningAtZ{1} = lookup_selector_at_z{2} /\
+            proofLookupTableTypePolyOpeningAtZ{1} = table_type_at_z{2} /\
+            proofLookupSPolyOpeningAtZOmega{1} = s_at_z_omega{2} /\
+            proofLookupGrandProductOpeningAtZOmega{1} = z_lookup_at_z_omega{2} /\
+            proofLookupTPolyOpeningAtZOmega{1} = t_at_z_omega{2} /\
+            proofLinearisationPolyOpeningAtZ{1} = r_at_z{2} /\
+            proofQuotientPolyParts0{1} = t_0{2} /\
+            proofQuotientPolyParts1{1} = t_1{2} /\
+            proofQuotientPolyParts2{1} = t_2{2} /\
+            proofQuotientPolyParts3{1} = t_3{2} /\
+            state{2} = (state0_14{1}, state1_14{1}) /\
+            stateAlpha{1} = alpha{2} /\
+            stateBeta{1} = beta_{2} /\
+            stateGamma{1} = gamma{2} /\
+            stateBetaLookup{1} = beta'{2} /\
+            stateGammaLookup{1} = gamma'{2} /\
+            stateEta{1} = eta_{2}            
+          ).
+            wp. skip. rewrite /commit_fr /commit_g. by progress.
+
+          seq 17 2: (
+            !failed{1} /\
+            isValid{2} /\
+            !vk_recursive_flag{1} /\
+            _public_input{1} = public_input{2} /\
+            _state_poly_0{1} = a{2} /\
+            _state_poly_1{1} = b{2} /\
+            _state_poly_2{1} = c{2} /\
+            _state_poly_3{1} = d{2} /\
+            _copy_permutation_grand_product{1} = z_perm{2} /\
+            _lookup_s_poly{1} = s{2} /\
+            _lookup_grand_product{1} = z_lookup{2} /\
+            _quotient_poly_part_0{1} = t_0{2} /\
+            _quotient_poly_part_1{1} = t_1{2} /\
+            _quotient_poly_part_2{1} = t_2{2} /\
+            _quotient_poly_part_3{1} = t_3{2} /\
+            _state_poly_0_opening_at_z{1} = a_at_z{2} /\
+            _state_poly_1_opening_at_z{1} = b_at_z{2} /\
+            _state_poly_2_opening_at_z{1} = c_at_z{2} /\
+            _state_poly_3_opening_at_z{1} = d_at_z{2} /\
+            _state_poly_3_opening_at_z_omega{1} = d_at_z_omega{2} /\
+            _gate_selector_0_opening_at_z{1} = main_gate_selector_at_z{2} /\
+            _copy_permutation_poly_0_opening_at_z{1} = sigma_0_at_z{2} /\
+            _copy_permutation_poly_1_opening_at_z{1} = sigma_1_at_z{2} /\
+            _copy_permutation_poly_2_opening_at_z{1} = sigma_2_at_z{2} /\
+            _copy_permutation_grand_product_opening_at_z_omega{1} = z_perm_at_z_omega{2} /\
+            _lookup_s_poly_opening_at_z_omega{1} = s_at_z_omega{2} /\
+            _lookup_grand_product_opening_at_z_omega{1} = z_lookup_at_z_omega{2} /\
+            _lookup_t_poly_opening_at_z{1} = t_at_z{2} /\
+            _lookup_t_poly_opening_at_z_omega{1} = t_at_z_omega{2} /\
+            _lookup_selector_poly_opening_at_z{1} = lookup_selector_at_z{2} /\
+            _lookup_table_type_poly_opening_at_z{1} = table_type_at_z{2} /\
+            _quotient_poly_opening_at_z{1} = quotient_poly_opening_at_z{2} /\
+            _linearisation_poly_opening_at_z{1} = r_at_z{2} /\
+            _opening_proof_at_z{1} = w{2} /\
+            _opening_proof_at_z_omega{1} = w'{2} /\
+            _recursive_part_p1{1} = None /\
+            _recursive_part_p2{1} = None /\
+            k0{2} = (FieldR.inF Constants.NON_RESIDUE_0) /\
+            k1{2} = (FieldR.inF Constants.NON_RESIDUE_1) /\
+            k2{2} = (FieldR.inF Constants.NON_RESIDUE_2) /\
+            n{2} = Constants.DOMAIN_SIZE /\
+            q_a{2} = vk_gate_setup_0 /\
+            q_b{2} = vk_gate_setup_1 /\
+            q_c{2} = vk_gate_setup_2 /\
+            q_d{2} = vk_gate_setup_3 /\
+            q_ab{2} = vk_gate_setup_4 /\
+            q_ac{2} = vk_gate_setup_5 /\
+            q_const{2} = vk_gate_setup_6 /\
+            q_d_next{2} = vk_gate_setup_7 /\
+            custom_gate_selector{2} = vk_gate_selectors_1 /\
+            sigma_0{2} = vk_permutation_0 /\
+            sigma_1{2} = vk_permutation_1 /\
+            sigma_2{2} = vk_permutation_2 /\
+            sigma_3{2} = vk_permutation_3 /\
+            lookup_selector{2} = vk_lookup_selector /\
+            table_type{2} = vk_lookup_table_type /\
+            omega{2} = Constants.OMEGAFr /\
+            col_0{2} = vk_lookup_table_0 /\
+            col_1{2} = vk_lookup_table_1 /\
+            col_2{2} = vk_lookup_table_2 /\
+            col_3{2} = vk_lookup_table_3 /\
+            n{2} = Constants.DOMAIN_SIZE /\
+            proofOpeningProofAtZ{1} = w{2} /\
+            proofOpeningProofAtZOmega{1} = w'{2} /\
+            proofQuotientPolyOpeningAtZ{1} = quotient_poly_opening_at_z{2} /\
+            proofStatePolys0OpeningAtZ{1} = a_at_z{2} /\
+            proofStatePolys1OpeningAtZ{1} = b_at_z{2} /\
+            proofStatePolys2OpeningAtZ{1} = c_at_z{2} /\
+            proofStatePolys3OpeningAtZ{1} = d_at_z{2} /\
+            proofStatePolys3OpeningAtZOmega{1} = d_at_z_omega{2} /\
+            proofGateSelectors0OpeningAtZ{1} = main_gate_selector_at_z{2} /\
+            proofCopyPermutationPolys0OpeningAtZ{1} = sigma_0_at_z{2} /\
+            proofCopyPermutationPolys1OpeningAtZ{1} = sigma_1_at_z{2} /\
+            proofCopyPermutationPolys2OpeningAtZ{1} = sigma_2_at_z{2} /\
+            proofCopyPermutationGrandProductOpeningAtZOmega{1} = z_perm_at_z_omega{2} /\
+            proofLookupTPolyOpeningAtZ{1} = t_at_z{2} /\
+            proofLookupSelectorPolyOpeningAtZ{1} = lookup_selector_at_z{2} /\
+            proofLookupTableTypePolyOpeningAtZ{1} = table_type_at_z{2} /\
+            proofLookupSPolyOpeningAtZOmega{1} = s_at_z_omega{2} /\
+            proofLookupGrandProductOpeningAtZOmega{1} = z_lookup_at_z_omega{2} /\
+            proofLookupTPolyOpeningAtZOmega{1} = t_at_z_omega{2} /\
+            proofLinearisationPolyOpeningAtZ{1} = r_at_z{2} /\
+            state{2} = (state0_22{1}, state1_22{1}) /\
+            stateAlpha{1} = alpha{2} /\
+            stateBeta{1} = beta_{2} /\
+            stateGamma{1} = gamma{2} /\
+            stateBetaLookup{1} = beta'{2} /\
+            stateGammaLookup{1} = gamma'{2} /\
+            stateEta{1} = eta_{2} /\
+            stateZ{1} = z{2}
+          ).
+            wp. skip. rewrite /commit_fr /commit_g. by progress.
+
+          seq 1 0: (
+            #pre /\
+            stateZInDomain{1} = z{2} ^ n{2}
+          ).
+            wp. skip. by progress.
+
+          seq 6 0: (
+            #pre /\
+            (state0_25{1}, state1_25{1}) = commit_fr(commit_fr(commit_fr state{2} quotient_poly_opening_at_z{2}) a_at_z{2}) b_at_z{2}
+          ).
+            wp. skip. by progress.
+
+          seq 6 0: (
+            #pre /\
+            (state0_28{1}, state1_28{1}) = commit_fr(commit_fr(commit_fr(commit_fr(commit_fr(commit_fr state{2} quotient_poly_opening_at_z{2}) a_at_z{2}) b_at_z{2}) c_at_z{2}) d_at_z{2}) d_at_z_omega{2}
+          ).
+            wp. skip. progress.
+            rewrite -H2 /commit_fr.
+            reflexivity.
+
+          seq 6 0: (
+            #pre /\
+            (state0_31{1}, state1_31{1}) = commit_fr(commit_fr(commit_fr(commit_fr(commit_fr(commit_fr(commit_fr(commit_fr(commit_fr state{2} quotient_poly_opening_at_z{2}) a_at_z{2}) b_at_z{2}) c_at_z{2}) d_at_z{2}) d_at_z_omega{2}) main_gate_selector_at_z{2}) sigma_0_at_z{2}) sigma_1_at_z{2}
+          ).
+            wp. skip. progress.
+            rewrite -H3 /commit_fr.
+            reflexivity.
+
+          seq 6 0: (
+            #pre /\
+            (state0_34{1}, state1_34{1}) = commit_fr(commit_fr(commit_fr(commit_fr(commit_fr(commit_fr(commit_fr(commit_fr(commit_fr(commit_fr(commit_fr(commit_fr state{2} quotient_poly_opening_at_z{2}) a_at_z{2}) b_at_z{2}) c_at_z{2}) d_at_z{2}) d_at_z_omega{2}) main_gate_selector_at_z{2}) sigma_0_at_z{2}) sigma_1_at_z{2}) sigma_2_at_z{2}) z_perm_at_z_omega{2}) t_at_z{2}
+          ).
+            wp. skip. progress.
+            rewrite -H4 /commit_fr.
+            reflexivity.
+
+          seq 6 0: (
+            #pre /\
+            (state0_37{1}, state1_37{1}) = commit_fr(commit_fr(commit_fr( commit_fr(commit_fr(commit_fr(commit_fr(commit_fr(commit_fr(commit_fr(commit_fr(commit_fr(commit_fr(commit_fr(commit_fr state{2} quotient_poly_opening_at_z{2}) a_at_z{2}) b_at_z{2}) c_at_z{2}) d_at_z{2}) d_at_z_omega{2}) main_gate_selector_at_z{2}) sigma_0_at_z{2}) sigma_1_at_z{2}) sigma_2_at_z{2}) z_perm_at_z_omega{2}) t_at_z{2}) lookup_selector_at_z{2}) table_type_at_z{2} ) s_at_z_omega{2}
+          ).
+            wp. skip. progress.
+            rewrite -H5 /commit_fr.
+            reflexivity.
+
+          seq 6 0: (
+            #pre /\
+            (state0_40{1}, state1_40{1}) = commit_fr(commit_fr(commit_fr(commit_fr(commit_fr(commit_fr(commit_fr(commit_fr(commit_fr(commit_fr(commit_fr(commit_fr(commit_fr(commit_fr(commit_fr(commit_fr(commit_fr(commit_fr state{2} quotient_poly_opening_at_z{2}) a_at_z{2}) b_at_z{2}) c_at_z{2}) d_at_z{2}) d_at_z_omega{2}) main_gate_selector_at_z{2}) sigma_0_at_z{2}) sigma_1_at_z{2}) sigma_2_at_z{2}) z_perm_at_z_omega{2}) t_at_z{2}) lookup_selector_at_z{2}) table_type_at_z{2}) s_at_z_omega{2}) z_lookup_at_z_omega{2}) t_at_z_omega{2}) r_at_z{2}
+          ).
+            wp. skip. progress.
+            rewrite -H6 /commit_fr.
+            reflexivity.
+
+          seq 1 2: (
+            !failed{1} /\
+            isValid{2} /\
+            !vk_recursive_flag{1} /\
+            _public_input{1} = public_input{2} /\
+            _state_poly_0{1} = a{2} /\
+            _state_poly_1{1} = b{2} /\
+            _state_poly_2{1} = c{2} /\
+            _state_poly_3{1} = d{2} /\
+            _copy_permutation_grand_product{1} = z_perm{2} /\
+            _lookup_s_poly{1} = s{2} /\
+            _lookup_grand_product{1} = z_lookup{2} /\
+            _quotient_poly_part_0{1} = t_0{2} /\
+            _quotient_poly_part_1{1} = t_1{2} /\
+            _quotient_poly_part_2{1} = t_2{2} /\
+            _quotient_poly_part_3{1} = t_3{2} /\
+            _state_poly_0_opening_at_z{1} = a_at_z{2} /\
+            _state_poly_1_opening_at_z{1} = b_at_z{2} /\
+            _state_poly_2_opening_at_z{1} = c_at_z{2} /\
+            _state_poly_3_opening_at_z{1} = d_at_z{2} /\
+            _state_poly_3_opening_at_z_omega{1} = d_at_z_omega{2} /\
+            _gate_selector_0_opening_at_z{1} = main_gate_selector_at_z{2} /\
+            _copy_permutation_poly_0_opening_at_z{1} = sigma_0_at_z{2} /\
+            _copy_permutation_poly_1_opening_at_z{1} = sigma_1_at_z{2} /\
+            _copy_permutation_poly_2_opening_at_z{1} = sigma_2_at_z{2} /\
+            _copy_permutation_grand_product_opening_at_z_omega{1} = z_perm_at_z_omega{2} /\
+            _lookup_s_poly_opening_at_z_omega{1} = s_at_z_omega{2} /\
+            _lookup_grand_product_opening_at_z_omega{1} = z_lookup_at_z_omega{2} /\
+            _lookup_t_poly_opening_at_z{1} = t_at_z{2} /\
+            _lookup_t_poly_opening_at_z_omega{1} = t_at_z_omega{2} /\
+            _lookup_selector_poly_opening_at_z{1} = lookup_selector_at_z{2} /\
+            _lookup_table_type_poly_opening_at_z{1} = table_type_at_z{2} /\
+            _quotient_poly_opening_at_z{1} = quotient_poly_opening_at_z{2} /\
+            _linearisation_poly_opening_at_z{1} = r_at_z{2} /\
+            _opening_proof_at_z{1} = w{2} /\
+            _opening_proof_at_z_omega{1} = w'{2} /\
+            _recursive_part_p1{1} = None /\
+            _recursive_part_p2{1} = None /\
+            k0{2} = (FieldR.inF Constants.NON_RESIDUE_0) /\
+            k1{2} = (FieldR.inF Constants.NON_RESIDUE_1) /\
+            k2{2} = (FieldR.inF Constants.NON_RESIDUE_2) /\
+            n{2} = Constants.DOMAIN_SIZE /\
+            q_a{2} = vk_gate_setup_0 /\
+            q_b{2} = vk_gate_setup_1 /\
+            q_c{2} = vk_gate_setup_2 /\
+            q_d{2} = vk_gate_setup_3 /\
+            q_ab{2} = vk_gate_setup_4 /\
+            q_ac{2} = vk_gate_setup_5 /\
+            q_const{2} = vk_gate_setup_6 /\
+            q_d_next{2} = vk_gate_setup_7 /\
+            custom_gate_selector{2} = vk_gate_selectors_1 /\
+            sigma_0{2} = vk_permutation_0 /\
+            sigma_1{2} = vk_permutation_1 /\
+            sigma_2{2} = vk_permutation_2 /\
+            sigma_3{2} = vk_permutation_3 /\
+            lookup_selector{2} = vk_lookup_selector /\
+            table_type{2} = vk_lookup_table_type /\
+            omega{2} = Constants.OMEGAFr /\
+            col_0{2} = vk_lookup_table_0 /\
+            col_1{2} = vk_lookup_table_1 /\
+            col_2{2} = vk_lookup_table_2 /\
+            col_3{2} = vk_lookup_table_3 /\
+            state{2} = (state0_40{1}, state1_40{1}) /\
+            proofOpeningProofAtZ{1} = w{2} /\
+            proofOpeningProofAtZOmega{1} = w'{2} /\
+            state{2} = (state0_40{1}, state1_40{1}) /\
+            stateAlpha{1} = alpha{2} /\
+            stateBeta{1} = beta_{2} /\
+            stateGamma{1} = gamma{2} /\
+            stateBetaLookup{1} = beta'{2} /\
+            stateGammaLookup{1} = gamma'{2} /\
+            stateEta{1} = eta_{2} /\
+            stateZ{1} = z{2} /\
+            stateZInDomain{1} = z{2} ^ n{2} /\
+            stateV{1} = v{2}
+          ).
+            wp. skip. progress. rewrite H7. reflexivity.
+            rewrite -H7. by progress.
+            rewrite -H7 /get_commitment. by progress.
+
+          wp. skip. progress. right. by progress.
+      (* initialize transcript done *)
+
+      (* verify quotient evaluation *)
+      seq 2 4: (
+        (failed{1} /\ !isValid{2}) \/ (
+        !failed{1} /\ isValid{2} /\
+        !vk_recursive_flag{1} /\
+        _public_input{1} = public_input{2} /\
+        _state_poly_0{1} = a{2} /\
+        _state_poly_1{1} = b{2} /\
+        _state_poly_2{1} = c{2} /\
+        _state_poly_3{1} = d{2} /\
+        _copy_permutation_grand_product{1} = z_perm{2} /\
+        _lookup_s_poly{1} = s{2} /\
+        _lookup_grand_product{1} = z_lookup{2} /\
+        _quotient_poly_part_0{1} = t_0{2} /\
+        _quotient_poly_part_1{1} = t_1{2} /\
+        _quotient_poly_part_2{1} = t_2{2} /\
+        _quotient_poly_part_3{1} = t_3{2} /\
+        _state_poly_0_opening_at_z{1} = a_at_z{2} /\
+        _state_poly_1_opening_at_z{1} = b_at_z{2} /\
+        _state_poly_2_opening_at_z{1} = c_at_z{2} /\
+        _state_poly_3_opening_at_z{1} = d_at_z{2} /\
+        _state_poly_3_opening_at_z_omega{1} = d_at_z_omega{2} /\
+        _gate_selector_0_opening_at_z{1} = main_gate_selector_at_z{2} /\
+        _copy_permutation_poly_0_opening_at_z{1} = sigma_0_at_z{2} /\
+        _copy_permutation_poly_1_opening_at_z{1} = sigma_1_at_z{2} /\ 
+        _copy_permutation_poly_2_opening_at_z{1} = sigma_2_at_z{2} /\
+        _copy_permutation_grand_product_opening_at_z_omega{1} = z_perm_at_z_omega{2} /\
+        _lookup_s_poly_opening_at_z_omega{1} = s_at_z_omega{2} /\
+        _lookup_grand_product_opening_at_z_omega{1} = z_lookup_at_z_omega{2} /\
+        _lookup_t_poly_opening_at_z{1} = t_at_z{2} /\
+        _lookup_t_poly_opening_at_z_omega{1} = t_at_z_omega{2} /\
+        _lookup_selector_poly_opening_at_z{1} = lookup_selector_at_z{2} /\
+        _lookup_table_type_poly_opening_at_z{1} = table_type_at_z{2} /\
+        _quotient_poly_opening_at_z{1} = quotient_poly_opening_at_z{2} /\
+        _linearisation_poly_opening_at_z{1} = r_at_z{2} /\
+        _opening_proof_at_z{1} = w{2} /\
+        _opening_proof_at_z_omega{1} = w'{2} /\
+        _recursive_part_p1{1} = None /\
+        _recursive_part_p2{1} = None /\
+        k0{2} = FieldR.inF Constants.NON_RESIDUE_0 /\
+        k1{2} = FieldR.inF Constants.NON_RESIDUE_1 /\ 
+        k2{2} = FieldR.inF Constants.NON_RESIDUE_2 /\
+        n{2} = Constants.DOMAIN_SIZE /\
+        q_a{2} = vk_gate_setup_0 /\
+        q_b{2} = vk_gate_setup_1 /\
+        q_c{2} = vk_gate_setup_2 /\
+        q_d{2} = vk_gate_setup_3 /\
+        q_ab{2} = vk_gate_setup_4 /\
+        q_ac{2} = vk_gate_setup_5 /\
+        q_const{2} = vk_gate_setup_6 /\
+        q_d_next{2} = vk_gate_setup_7 /\
+        custom_gate_selector{2} = vk_gate_selectors_1 /\
+        sigma_0{2} = vk_permutation_0 /\
+        sigma_1{2} = vk_permutation_1 /\
+        sigma_2{2} = vk_permutation_2 /\ 
+        sigma_3{2} = vk_permutation_3 /\
+        lookup_selector{2} = vk_lookup_selector /\
+        table_type{2} = vk_lookup_table_type /\
+        omega{2} = Constants.OMEGAFr /\
+        col_0{2} = vk_lookup_table_0 /\
+        col_1{2} = vk_lookup_table_1 /\
+        col_2{2} = vk_lookup_table_2 /\
+        col_3{2} = vk_lookup_table_3 /\
+        state_alpha{1} = alpha{2} /\
+        state_beta{1} = beta_{2} /\
+        state_beta_lookup{1} = beta'{2} /\
+        state_gamma{1} = gamma{2} /\
+        state_gamma_lookup{1} = gamma'{2} /\
+        state_eta{1} = eta_{2} /\
+        state_z{1} = z{2} /\
+        state_z_in_domain{1} = z{2} ^ n{2} /\
+        state_v{1} = v{2} /\
+        state_u{1} = u{2} /\
+        alpha2{1} = alpha{2}^2 /\
+        alpha3{1} = alpha{2}^3 /\
+        alpha4{1} = alpha{2}^4 /\
+        alpha5{1} = alpha{2}^5 /\
+        alpha6{1} = alpha{2}^6 /\
+        alpha7{1} = alpha{2}^7 /\
+        alpha8{1} = alpha{2}^8 /\
+        l0_at_z{1} = l_0_at_z{2} /\
+        ln_minus_one_at_z{1} = l_n_minus_one_at_z{2} /\
+        beta_plus_one{1} = FieldR.one + beta'{2} /\
+        beta_gamma_plus_gamma{1} = gamma'{2} * (FieldR.one + beta'{2}) /\
+        z_minus_last_omega{1} = z{2} - omega{2}^(n{2} - 1)
+      )).
+        case (failed{1}).
+        conseq (_: (failed{1} /\ !isValid{2}) ==> (failed{1} /\ !isValid{2})).
+          progress. by case H; progress.
+          progress. left. by progress.
+          inline VerifyQuotientEvaluation.high.
+          wp. skip. progress.
+            rewrite H0. by progress.
+            left. assumption.
+            rewrite H0. by progress.
+
+        (* case !failed{1} *)
+          inline VerifyQuotientEvaluation.high.
+          case (z{2} ^ Constants.DOMAIN_SIZE = FieldR.one).
+            rcondt{1} 22. progress.
+            wp. skip. progress. by case H; progress.
+            wp. skip. progress. rewrite H1. by progress.
+
+          (* case z{2} ^ Constants.DOMAIN_SIZE = FieldR.one *)
+            rcondf{1} 22. progress.
+            wp. skip. progress. by case H; progress.      
+            wp. skip. progress. rewrite H0 H1. case H. by progress.
+            progress. rewrite H2 H3. progress.
+            have ->: beta'{2} + FieldR.one = FieldR.one + beta'{2} by exact FieldR.ZModule.addrC.
+            have ->: gamma'{2} * beta'{2} + gamma'{2} = gamma'{2} * (FieldR.one + beta'{2}) by
+              rewrite (FieldR.ZrRing.mulrC _ (FieldR.one + _));
+              rewrite FieldR.ComRing.mulrDl;
+              rewrite FieldR.ComRing.mul1r;
+              rewrite FieldR.ZModule.addrC;
+              rewrite FieldR.ZrRing.mulrC;
+              reflexivity.
+            progress.
+            pose a8 := FieldR.( * ) (FieldR.( * ) (alpha{2}^8)  _) _.
+            pose a7 := FieldR.( * ) (alpha{2}^7)  _.
+            pose a6 := FieldR.( * ) (FieldR.( * ) (FieldR.( * ) (alpha{2}^6)  _) _) _.
+            have ->: alpha{2} ^ 6 *
+              (s_at_z_omega{2} * beta'{2} + gamma'{2} * (FieldR.one + beta'{2})) *
+              (z{2} + - Constants.OMEGAFr ^ (Constants.DOMAIN_SIZE - 1)) *
+              z_lookup_at_z_omega{2} = a6 by
+                pose x1 := alpha{2}^6 * (s_at_z_omega{2} * beta'{2} + gamma'{2} * (FieldR.one + beta'{2}));
+                pose x2 := (z{2} + - Constants.OMEGAFr ^ (Constants.DOMAIN_SIZE - 1));
+                rewrite -FieldR.ComRing.mulrA;
+                rewrite (FieldR.ZrRing.mulrC x2);
+                rewrite FieldR.ComRing.mulrA;
+                progress.
+            pose a5 := FieldR.( * ) (alpha{2}^5)  _.
+            pose a4 := FieldR.( * ) (FieldR.( * ) (FieldR.( * ) (FieldR.( * ) (FieldR.( * ) (alpha{2}^4)  _) _) _) _) _.
+            pose y1 := quotient_poly_opening_at_z{2} * (z{2} ^ Constants.DOMAIN_SIZE + -FieldR.one).
+            pose y2 := FieldR.( + ) _ _.
+            case (y1 = y2); by progress.
+
+      (* verify quotient evaluation done *)
+
+      (* prepare queries *)
+      seq 1 4: (
+        (failed{1} /\ !isValid{2}) \/ (
+        !failed{1} /\ isValid{2} /\
+        !vk_recursive_flag{1} /\
+        _public_input{1} = public_input{2} /\
+        _state_poly_0{1} = a{2} /\
+        _state_poly_1{1} = b{2} /\
+        _state_poly_2{1} = c{2} /\
+        _state_poly_3{1} = d{2} /\
+        _copy_permutation_grand_product{1} = z_perm{2} /\
+        _lookup_s_poly{1} = s{2} /\
+        _lookup_grand_product{1} = z_lookup{2} /\
+        _quotient_poly_part_0{1} = t_0{2} /\
+        _quotient_poly_part_1{1} = t_1{2} /\
+        _quotient_poly_part_2{1} = t_2{2} /\
+        _quotient_poly_part_3{1} = t_3{2} /\
+        _state_poly_0_opening_at_z{1} = a_at_z{2} /\
+        _state_poly_1_opening_at_z{1} = b_at_z{2} /\
+        _state_poly_2_opening_at_z{1} = c_at_z{2} /\
+        _state_poly_3_opening_at_z{1} = d_at_z{2} /\
+        _state_poly_3_opening_at_z_omega{1} = d_at_z_omega{2} /\
+        _gate_selector_0_opening_at_z{1} = main_gate_selector_at_z{2} /\
+        _copy_permutation_poly_0_opening_at_z{1} = sigma_0_at_z{2} /\
+        _copy_permutation_poly_1_opening_at_z{1} = sigma_1_at_z{2} /\ 
+        _copy_permutation_poly_2_opening_at_z{1} = sigma_2_at_z{2} /\
+        _copy_permutation_grand_product_opening_at_z_omega{1} = z_perm_at_z_omega{2} /\
+        _lookup_s_poly_opening_at_z_omega{1} = s_at_z_omega{2} /\
+        _lookup_grand_product_opening_at_z_omega{1} = z_lookup_at_z_omega{2} /\
+        _lookup_t_poly_opening_at_z{1} = t_at_z{2} /\
+        _lookup_t_poly_opening_at_z_omega{1} = t_at_z_omega{2} /\
+        _lookup_selector_poly_opening_at_z{1} = lookup_selector_at_z{2} /\
+        _lookup_table_type_poly_opening_at_z{1} = table_type_at_z{2} /\
+        _quotient_poly_opening_at_z{1} = quotient_poly_opening_at_z{2} /\
+        _linearisation_poly_opening_at_z{1} = r_at_z{2} /\
+        _opening_proof_at_z{1} = w{2} /\
+        _opening_proof_at_z_omega{1} = w'{2} /\
+        _recursive_part_p1{1} = None /\
+        _recursive_part_p2{1} = None /\
+        k0{2} = FieldR.inF Constants.NON_RESIDUE_0 /\
+        k1{2} = FieldR.inF Constants.NON_RESIDUE_1 /\ 
+        k2{2} = FieldR.inF Constants.NON_RESIDUE_2 /\
+        n{2} = Constants.DOMAIN_SIZE /\
+        q_a{2} = vk_gate_setup_0 /\
+        q_b{2} = vk_gate_setup_1 /\
+        q_c{2} = vk_gate_setup_2 /\
+        q_d{2} = vk_gate_setup_3 /\
+        q_ab{2} = vk_gate_setup_4 /\
+        q_ac{2} = vk_gate_setup_5 /\
+        q_const{2} = vk_gate_setup_6 /\
+        q_d_next{2} = vk_gate_setup_7 /\
+        custom_gate_selector{2} = vk_gate_selectors_1 /\
+        sigma_0{2} = vk_permutation_0 /\
+        sigma_1{2} = vk_permutation_1 /\
+        sigma_2{2} = vk_permutation_2 /\ 
+        sigma_3{2} = vk_permutation_3 /\
+        lookup_selector{2} = vk_lookup_selector /\
+        table_type{2} = vk_lookup_table_type /\
+        omega{2} = Constants.OMEGAFr /\
+        col_0{2} = vk_lookup_table_0 /\
+        col_1{2} = vk_lookup_table_1 /\
+        col_2{2} = vk_lookup_table_2 /\
+        col_3{2} = vk_lookup_table_3 /\
+        state_alpha{1} = alpha{2} /\
+        state_beta{1} = beta_{2} /\
+        state_beta_lookup{1} = beta'{2} /\
+        state_gamma{1} = gamma{2} /\
+        state_gamma_lookup{1} = gamma'{2} /\
+        state_eta{1} = eta_{2} /\
+        state_z{1} = z{2} /\
+        state_z_in_domain{1} = z{2} ^ n{2} /\
+        state_v{1} = v{2} /\
+        state_u{1} = u{2} /\
+        alpha2{1} = alpha{2}^2 /\
+        alpha3{1} = alpha{2}^3 /\
+        alpha4{1} = alpha{2}^4 /\
+        alpha5{1} = alpha{2}^5 /\
+        alpha6{1} = alpha{2}^6 /\
+        alpha7{1} = alpha{2}^7 /\
+        alpha8{1} = alpha{2}^8 /\
+        l0_at_z{1} = l_0_at_z{2} /\
+        ln_minus_one_at_z{1} = l_n_minus_one_at_z{2} /\
+        beta_plus_one{1} = FieldR.one + beta'{2} /\
+        beta_gamma_plus_gamma{1} = gamma'{2} * (FieldR.one + beta'{2}) /\
+        z_minus_last_omega{1} = z{2} - omega{2}^(n{2} - 1) /\
+        query_at_z_0{1} = d0{2} /\
+        query_at_z_1{1} = v{2} * (
+          main_gate_selector_at_z{2} * (
+            (a_at_z{2} * q_a{2}) +
+            (b_at_z{2} * q_b{2}) +
+            (c_at_z{2} * q_c{2}) +
+            (d_at_z{2} * q_d{2}) +
+            (a_at_z{2} * b_at_z{2} * q_ab{2}) +
+            (a_at_z{2} * c_at_z{2} * q_ac{2}) +
+            q_const{2} +
+            (d_at_z_omega{2} * q_d_next{2})
+          ) + 
+          alpha{2} * (
+            (
+              (a_at_z{2}^2 - b_at_z{2}) +
+              (b_at_z{2}^2 - c_at_z{2}) * alpha{2} +
+              (a_at_z{2} * c_at_z{2} - d_at_z{2}) * alpha{2}^2
+            )
+          )* custom_gate_selector{2} +
+          G.inv (alpha{2}^4 * z_perm_at_z_omega{2} * beta_{2} *
+            (sigma_0_at_z{2} * beta_{2} + gamma{2} + a_at_z{2}) *
+            (sigma_1_at_z{2} * beta_{2} + gamma{2} + b_at_z{2}) *
+            (sigma_2_at_z{2} * beta_{2} + gamma{2} + c_at_z{2}) *
+            sigma_3{2})
+          ) /\
+        copy_permutation_first_aggregated_commitment_coeff{1} = (                                
+          alpha{2}^4 * (z{2} * beta_{2} + gamma{2} + a_at_z{2}) *                               
+          (z{2} * beta_{2} * k0{2} + gamma{2} + b_at_z{2}) * 
+          (z{2} * beta_{2} * k1{2} + gamma{2} + c_at_z{2}) * 
+          (z{2} * beta_{2} * k2{2} + gamma{2} + d_at_z{2}) + 
+          l_0_at_z{2} * alpha{2}^5
+        ) * v{2} /\
+        lookupSFirstAggregatedCommitment{1} = v{2} * alpha{2}^6 * z_lookup_at_z_omega{2} * (z{2} - omega{2}^(n{2}-1)) /\
+        lookupGrandProductFirstAggregatedCoefficient{1} = ((
+          - alpha{2}^6 * (FieldR.one + beta'{2}) * (gamma'{2} + f_at_z{2}) * (z{2} - omega{2}^(n{2}-1)) * (
+            gamma'{2}*(FieldR.one + beta'{2}) + t_at_z{2} + beta'{2} * t_at_z_omega{2}
+          )) +
+          alpha{2}^7 * l_0_at_z{2} +
+          alpha{2}^8 * l_n_minus_one_at_z{2}) * v{2} /\
+        query_t_poly_aggregated{1} = t{2} /\
+        d1{2} = main_gate_selector_at_z{2} * (
+            (a_at_z{2} * q_a{2}) +
+            (b_at_z{2} * q_b{2}) +
+            (c_at_z{2} * q_c{2}) +
+            (d_at_z{2} * q_d{2}) +
+            (a_at_z{2} * b_at_z{2} * q_ab{2}) +
+            (a_at_z{2} * c_at_z{2} * q_ac{2}) +
+            q_const{2} +
+            (d_at_z_omega{2} * q_d_next{2})
+        ) 
+        + alpha{2} * (
+          (
+            (a_at_z{2}^2 - b_at_z{2}) +
+            (b_at_z{2}^2 - c_at_z{2}) * alpha{2} +
+            (a_at_z{2} * c_at_z{2} - d_at_z{2}) * alpha{2}^2
+          )
+        )* custom_gate_selector{2}
+        + alpha{2}^4 *
+          (a_at_z{2} + beta_{2} * z{2}         + gamma{2}) *                               
+          (b_at_z{2} + beta_{2} * z{2} * k0{2} + gamma{2}) * 
+          (c_at_z{2} + beta_{2} * z{2} * k1{2} + gamma{2}) * 
+          (d_at_z{2} + beta_{2} * z{2} * k2{2} + gamma{2}) * z_perm{2}
+        + G.inv (alpha{2}^4 * z_perm_at_z_omega{2} * beta_{2} *
+          (a_at_z{2} + beta_{2} * sigma_0_at_z{2} + gamma{2}) *
+          (b_at_z{2} + beta_{2} * sigma_1_at_z{2} + gamma{2}) *
+          (c_at_z{2} + beta_{2} * sigma_2_at_z{2} + gamma{2}) *
+          sigma_3{2})
+        + alpha{2}^5 * l_0_at_z{2} * z_perm{2}
+        + G.inv (alpha{2}^6 * (FieldR.one + beta'{2}) * (gamma'{2} + f_at_z{2}) * (z{2} - omega{2}^(n{2}-1)) *
+          (gamma'{2}*(FieldR.one + beta'{2}) + t_at_z{2} + beta'{2} * t_at_z_omega{2}) * z_lookup{2}
+        ) 
+          + alpha{2}^6 * z_lookup_at_z_omega{2} * (z{2} - omega{2}^(n{2}-1)) * s{2}
+          + alpha{2}^7 * l_0_at_z{2} * z_lookup{2}
+          + alpha{2}^8 * l_n_minus_one_at_z{2} * z_lookup{2}  /\
+        f_at_z{2} = lookup_selector_at_z{2} * (a_at_z{2} + eta_{2} * b_at_z{2} + eta_{2}^2 * c_at_z{2} + eta_{2}^3 * table_type_at_z{2})
+      )).
+        case (failed{1}).
+        conseq (_: (failed{1} /\ !isValid{2}) ==> (failed{1} /\ !isValid{2})).
+          progress. by case H; progress.
+          progress. left. by progress.
+          inline PrepareQueries.high.
+          wp. skip. by progress.
+
+        (* case failed{1} *)
+          transitivity{1} 
+            { (query_at_z_0, query_at_z_1, copy_permutation_first_aggregated_commitment_coeff, lookupSFirstAggregatedCommitment, lookupGrandProductFirstAggregatedCoefficient, query_t_poly_aggregated) <@ PrepareQueries.super_high(
+              state_alpha,
+              state_beta,
+              state_gamma,
+              state_v,
+              state_z,
+              Constants.DOMAIN_SIZE,
+              _quotient_poly_part_0,
+              _quotient_poly_part_1,
+              _quotient_poly_part_2,
+              _quotient_poly_part_3,
+              _gate_selector_0_opening_at_z,
+              _state_poly_0_opening_at_z,
+              _state_poly_1_opening_at_z,
+              _state_poly_2_opening_at_z,
+              _state_poly_3_opening_at_z,
+              vk_gate_setup_0,
+              vk_gate_setup_1,
+              vk_gate_setup_2,
+              vk_gate_setup_3,
+              vk_gate_setup_4,
+              vk_gate_setup_5,
+              vk_gate_setup_6,
+              vk_gate_setup_7,
+              _state_poly_3_opening_at_z_omega,
+              vk_gate_selectors_1,
+              _copy_permutation_grand_product_opening_at_z_omega,
+              _copy_permutation_poly_0_opening_at_z,
+              _copy_permutation_poly_1_opening_at_z,
+              _copy_permutation_poly_2_opening_at_z,
+              vk_permutation_3,
+              FieldR.inF Constants.NON_RESIDUE_0,
+              FieldR.inF Constants.NON_RESIDUE_1,
+              FieldR.inF Constants.NON_RESIDUE_2,
+              l0_at_z,
+              Constants.OMEGAFr, 
+              _lookup_grand_product_opening_at_z_omega,
+              vk_lookup_table_0,
+              vk_lookup_table_1,
+              vk_lookup_table_2,
+              vk_lookup_table_3,
+              state_eta,
+              _lookup_selector_poly_opening_at_z,
+              _lookup_table_type_poly_opening_at_z,
+              state_beta_lookup,
+              state_gamma_lookup,
+              _lookup_t_poly_opening_at_z,
+              _lookup_t_poly_opening_at_z_omega,
+              ln_minus_one_at_z
+            );} (
+              ={failed, _public_input, _state_poly_0, _state_poly_1, _state_poly_2, _state_poly_3, vk_recursive_flag ,_copy_permutation_grand_product, _lookup_s_poly, _lookup_grand_product, _quotient_poly_part_0, _quotient_poly_part_1, _quotient_poly_part_2, _quotient_poly_part_3, _state_poly_0_opening_at_z, _state_poly_1_opening_at_z, _state_poly_2_opening_at_z, _state_poly_3_opening_at_z, _state_poly_3_opening_at_z_omega, _gate_selector_0_opening_at_z, _copy_permutation_poly_0_opening_at_z, _copy_permutation_poly_1_opening_at_z, _copy_permutation_poly_2_opening_at_z, _copy_permutation_grand_product_opening_at_z_omega, _lookup_s_poly_opening_at_z_omega, _lookup_grand_product_opening_at_z_omega, _lookup_t_poly_opening_at_z, _lookup_t_poly_opening_at_z_omega, _lookup_selector_poly_opening_at_z, _lookup_table_type_poly_opening_at_z, _quotient_poly_opening_at_z, _linearisation_poly_opening_at_z, _opening_proof_at_z, _opening_proof_at_z_omega, _recursive_part_p1, _recursive_part_p2, state_alpha, state_beta, state_beta_lookup, state_gamma, state_gamma_lookup, state_eta, state_z, state_z_in_domain, state_v, state_u, alpha2, alpha3, alpha4, alpha5, alpha6, alpha7, alpha8, l0_at_z, ln_minus_one_at_z, beta_plus_one, beta_gamma_plus_gamma, z_minus_last_omega} /\
+              alpha2{1} = state_alpha{2}^2 /\
+              alpha3{1} = state_alpha{2}^3 /\
+              alpha4{1} = state_alpha{2}^4 /\
+              alpha5{1} = state_alpha{2}^5 /\
+              alpha6{1} = state_alpha{2}^6 /\
+              alpha7{1} = state_alpha{2}^7 /\
+              alpha8{1} = state_alpha{2}^8 /\ 
+              state_z_in_domain{1} = state_z{2} ^ Constants.DOMAIN_SIZE /\
+              z_minus_last_omega{1} = (state_z{2} - Constants.OMEGAFr^(Constants.DOMAIN_SIZE-1)) /\
+              beta_gamma_plus_gamma{1} = state_gamma_lookup{2}*(FieldR.one + state_beta_lookup{2}) /\
+              beta_plus_one{1} = (FieldR.one + state_beta_lookup{2})
+                 ==>
+              ={query_at_z_0, query_at_z_1, copy_permutation_first_aggregated_commitment_coeff, lookupSFirstAggregatedCommitment, lookupGrandProductFirstAggregatedCoefficient, query_t_poly_aggregated, failed, _public_input, _state_poly_0, _state_poly_1, _state_poly_2, _state_poly_3, vk_recursive_flag ,_copy_permutation_grand_product, _lookup_s_poly, _lookup_grand_product, _quotient_poly_part_0, _quotient_poly_part_1, _quotient_poly_part_2, _quotient_poly_part_3, _state_poly_0_opening_at_z, _state_poly_1_opening_at_z, _state_poly_2_opening_at_z, _state_poly_3_opening_at_z, _state_poly_3_opening_at_z_omega, _gate_selector_0_opening_at_z, _copy_permutation_poly_0_opening_at_z, _copy_permutation_poly_1_opening_at_z, _copy_permutation_poly_2_opening_at_z, _copy_permutation_grand_product_opening_at_z_omega, _lookup_s_poly_opening_at_z_omega, _lookup_grand_product_opening_at_z_omega, _lookup_t_poly_opening_at_z, _lookup_t_poly_opening_at_z_omega, _lookup_selector_poly_opening_at_z, _lookup_table_type_poly_opening_at_z, _quotient_poly_opening_at_z, _linearisation_poly_opening_at_z, _opening_proof_at_z, _opening_proof_at_z_omega, _recursive_part_p1, _recursive_part_p2, state_alpha, state_beta, state_beta_lookup, state_gamma, state_gamma_lookup, state_eta, state_z, state_z_in_domain, state_v, state_u, alpha2, alpha3, alpha4, alpha5, alpha6, alpha7, alpha8, l0_at_z, ln_minus_one_at_z, beta_plus_one, beta_gamma_plus_gamma, z_minus_last_omega}
+            ) (
+              !failed{1} /\
+              isValid{2} /\
+              !vk_recursive_flag{1} /\
+              _public_input{1} = public_input{2} /\
+              _state_poly_0{1} = a{2} /\
+              _state_poly_1{1} = b{2} /\
+              _state_poly_2{1} = c{2} /\
+              _state_poly_3{1} = d{2} /\
+              _copy_permutation_grand_product{1} = z_perm{2} /\
+              _lookup_s_poly{1} = s{2} /\
+              _lookup_grand_product{1} = z_lookup{2} /\
+              _quotient_poly_part_0{1} = t_0{2} /\
+              _quotient_poly_part_1{1} = t_1{2} /\
+              _quotient_poly_part_2{1} = t_2{2} /\
+              _quotient_poly_part_3{1} = t_3{2} /\
+              _state_poly_0_opening_at_z{1} = a_at_z{2} /\
+              _state_poly_1_opening_at_z{1} = b_at_z{2} /\
+              _state_poly_2_opening_at_z{1} = c_at_z{2} /\
+              _state_poly_3_opening_at_z{1} = d_at_z{2} /\
+              _state_poly_3_opening_at_z_omega{1} = d_at_z_omega{2} /\
+              _gate_selector_0_opening_at_z{1} = main_gate_selector_at_z{2} /\
+              _copy_permutation_poly_0_opening_at_z{1} = sigma_0_at_z{2} /\
+              _copy_permutation_poly_1_opening_at_z{1} = sigma_1_at_z{2} /\
+              _copy_permutation_poly_2_opening_at_z{1} = sigma_2_at_z{2} /\
+              _copy_permutation_grand_product_opening_at_z_omega{1} =
+              z_perm_at_z_omega{2} /\
+              _lookup_s_poly_opening_at_z_omega{1} = s_at_z_omega{2} /\
+              _lookup_grand_product_opening_at_z_omega{1} = z_lookup_at_z_omega{2} /\
+              _lookup_t_poly_opening_at_z{1} = t_at_z{2} /\
+              _lookup_t_poly_opening_at_z_omega{1} = t_at_z_omega{2} /\
+              _lookup_selector_poly_opening_at_z{1} = lookup_selector_at_z{2} /\
+              _lookup_table_type_poly_opening_at_z{1} = table_type_at_z{2} /\
+              _quotient_poly_opening_at_z{1} = quotient_poly_opening_at_z{2} /\
+              _linearisation_poly_opening_at_z{1} = r_at_z{2} /\
+              _opening_proof_at_z{1} = w{2} /\
+              _opening_proof_at_z_omega{1} = w'{2} /\
+              _recursive_part_p1{1} = None /\
+              _recursive_part_p2{1} = None /\
+              k0{2} = (FieldR.inF Constants.NON_RESIDUE_0) /\
+              k1{2} = (FieldR.inF Constants.NON_RESIDUE_1) /\
+              k2{2} = (FieldR.inF Constants.NON_RESIDUE_2) /\
+              n{2} = Constants.DOMAIN_SIZE /\
+              q_a{2} = vk_gate_setup_0 /\
+              q_b{2} = vk_gate_setup_1 /\
+              q_c{2} = vk_gate_setup_2 /\
+              q_d{2} = vk_gate_setup_3 /\
+              q_ab{2} = vk_gate_setup_4 /\
+              q_ac{2} = vk_gate_setup_5 /\
+              q_const{2} = vk_gate_setup_6 /\
+              q_d_next{2} = vk_gate_setup_7 /\
+              custom_gate_selector{2} = vk_gate_selectors_1 /\
+              sigma_0{2} = vk_permutation_0 /\
+              sigma_1{2} = vk_permutation_1 /\
+              sigma_2{2} = vk_permutation_2 /\
+              sigma_3{2} = vk_permutation_3 /\
+              lookup_selector{2} = vk_lookup_selector /\
+              table_type{2} = vk_lookup_table_type /\
+              omega{2} = Constants.OMEGAFr /\
+              col_0{2} = vk_lookup_table_0 /\
+              col_1{2} = vk_lookup_table_1 /\
+              col_2{2} = vk_lookup_table_2 /\
+              col_3{2} = vk_lookup_table_3 /\
+              state_alpha{1} = alpha{2} /\
+              state_beta{1} = beta_{2} /\
+              state_beta_lookup{1} = beta'{2} /\
+              state_gamma{1} = gamma{2} /\
+              state_gamma_lookup{1} = gamma'{2} /\
+              state_eta{1} = eta_{2} /\
+              state_z{1} = z{2} /\
+              state_z_in_domain{1} = z{2} ^ n{2} /\
+              state_v{1} = v{2} /\
+              state_u{1} = u{2} /\
+              alpha2{1} = alpha{2} ^ 2 /\
+              alpha3{1} = alpha{2} ^ 3 /\
+              alpha4{1} = alpha{2} ^ 4 /\
+              alpha5{1} = alpha{2} ^ 5 /\
+              alpha6{1} = alpha{2} ^ 6 /\
+              alpha7{1} = alpha{2} ^ 7 /\
+              alpha8{1} = alpha{2} ^ 8 /\
+              l0_at_z{1} = l_0_at_z{2} /\
+              ln_minus_one_at_z{1} = l_n_minus_one_at_z{2} /\
+              beta_plus_one{1} = FieldR.one + beta'{2} /\
+              beta_gamma_plus_gamma{1} = gamma'{2} * (FieldR.one + beta'{2}) /\
+              z_minus_last_omega{1} = z{2} - omega{2} ^ (n{2} - 1)
+                ==>
+              !failed{1} /\ isValid{2} /\
+              !vk_recursive_flag{1} /\
+              _public_input{1} = public_input{2} /\
+              _state_poly_0{1} = a{2} /\
+              _state_poly_1{1} = b{2} /\
+              _state_poly_2{1} = c{2} /\
+              _state_poly_3{1} = d{2} /\
+              _copy_permutation_grand_product{1} = z_perm{2} /\
+              _lookup_s_poly{1} = s{2} /\
+              _lookup_grand_product{1} = z_lookup{2} /\
+              _quotient_poly_part_0{1} = t_0{2} /\
+              _quotient_poly_part_1{1} = t_1{2} /\
+              _quotient_poly_part_2{1} = t_2{2} /\
+              _quotient_poly_part_3{1} = t_3{2} /\
+              _state_poly_0_opening_at_z{1} = a_at_z{2} /\
+              _state_poly_1_opening_at_z{1} = b_at_z{2} /\
+              _state_poly_2_opening_at_z{1} = c_at_z{2} /\
+              _state_poly_3_opening_at_z{1} = d_at_z{2} /\
+              _state_poly_3_opening_at_z_omega{1} = d_at_z_omega{2} /\
+              _gate_selector_0_opening_at_z{1} = main_gate_selector_at_z{2} /\
+              _copy_permutation_poly_0_opening_at_z{1} = sigma_0_at_z{2} /\
+              _copy_permutation_poly_1_opening_at_z{1} = sigma_1_at_z{2} /\ 
+              _copy_permutation_poly_2_opening_at_z{1} = sigma_2_at_z{2} /\
+              _copy_permutation_grand_product_opening_at_z_omega{1} = z_perm_at_z_omega{2} /\
+              _lookup_s_poly_opening_at_z_omega{1} = s_at_z_omega{2} /\
+              _lookup_grand_product_opening_at_z_omega{1} = z_lookup_at_z_omega{2} /\
+              _lookup_t_poly_opening_at_z{1} = t_at_z{2} /\
+              _lookup_t_poly_opening_at_z_omega{1} = t_at_z_omega{2} /\
+              _lookup_selector_poly_opening_at_z{1} = lookup_selector_at_z{2} /\
+              _lookup_table_type_poly_opening_at_z{1} = table_type_at_z{2} /\
+              _quotient_poly_opening_at_z{1} = quotient_poly_opening_at_z{2} /\
+              _linearisation_poly_opening_at_z{1} = r_at_z{2} /\
+              _opening_proof_at_z{1} = w{2} /\
+              _opening_proof_at_z_omega{1} = w'{2} /\
+              _recursive_part_p1{1} = None /\
+              _recursive_part_p2{1} = None /\
+              k0{2} = FieldR.inF Constants.NON_RESIDUE_0 /\
+              k1{2} = FieldR.inF Constants.NON_RESIDUE_1 /\ 
+              k2{2} = FieldR.inF Constants.NON_RESIDUE_2 /\
+              n{2} = Constants.DOMAIN_SIZE /\
+              q_a{2} = vk_gate_setup_0 /\
+              q_b{2} = vk_gate_setup_1 /\
+              q_c{2} = vk_gate_setup_2 /\
+              q_d{2} = vk_gate_setup_3 /\
+              q_ab{2} = vk_gate_setup_4 /\
+              q_ac{2} = vk_gate_setup_5 /\
+              q_const{2} = vk_gate_setup_6 /\
+              q_d_next{2} = vk_gate_setup_7 /\
+              custom_gate_selector{2} = vk_gate_selectors_1 /\
+              sigma_0{2} = vk_permutation_0 /\
+              sigma_1{2} = vk_permutation_1 /\
+              sigma_2{2} = vk_permutation_2 /\ 
+              sigma_3{2} = vk_permutation_3 /\
+              lookup_selector{2} = vk_lookup_selector /\
+              table_type{2} = vk_lookup_table_type /\
+              omega{2} = Constants.OMEGAFr /\
+              col_0{2} = vk_lookup_table_0 /\
+              col_1{2} = vk_lookup_table_1 /\
+              col_2{2} = vk_lookup_table_2 /\
+              col_3{2} = vk_lookup_table_3 /\
+              state_alpha{1} = alpha{2} /\
+              state_beta{1} = beta_{2} /\
+              state_beta_lookup{1} = beta'{2} /\
+              state_gamma{1} = gamma{2} /\
+              state_gamma_lookup{1} = gamma'{2} /\
+              state_eta{1} = eta_{2} /\
+              state_z{1} = z{2} /\
+              state_z_in_domain{1} = z{2} ^ n{2} /\
+              state_v{1} = v{2} /\
+              state_u{1} = u{2} /\
+              alpha2{1} = alpha{2}^2 /\
+              alpha3{1} = alpha{2}^3 /\
+              alpha4{1} = alpha{2}^4 /\
+              alpha5{1} = alpha{2}^5 /\
+              alpha6{1} = alpha{2}^6 /\
+              alpha7{1} = alpha{2}^7 /\
+              alpha8{1} = alpha{2}^8 /\
+              l0_at_z{1} = l_0_at_z{2} /\
+              ln_minus_one_at_z{1} = l_n_minus_one_at_z{2} /\
+              beta_plus_one{1} = FieldR.one + beta'{2} /\
+              beta_gamma_plus_gamma{1} = gamma'{2} * (FieldR.one + beta'{2}) /\
+              z_minus_last_omega{1} = z{2} - omega{2}^(n{2} - 1) /\
+              query_at_z_0{1} = d0{2} /\
+              query_at_z_1{1} = v{2} * (
+                main_gate_selector_at_z{2} * (
+                  (a_at_z{2} * q_a{2}) +
+                  (b_at_z{2} * q_b{2}) +
+                  (c_at_z{2} * q_c{2}) +
+                  (d_at_z{2} * q_d{2}) +
+                  (a_at_z{2} * b_at_z{2} * q_ab{2}) +
+                  (a_at_z{2} * c_at_z{2} * q_ac{2}) +
+                  q_const{2} +
+                  (d_at_z_omega{2} * q_d_next{2})
+                ) + 
+                alpha{2} * (
+                  (
+                    (a_at_z{2}^2 - b_at_z{2}) +
+                    (b_at_z{2}^2 - c_at_z{2}) * alpha{2} +
+                    (a_at_z{2} * c_at_z{2} - d_at_z{2}) * alpha{2}^2
+                  )
+                )* custom_gate_selector{2} +
+                G.inv (alpha{2}^4 * z_perm_at_z_omega{2} * beta_{2} *
+                  (sigma_0_at_z{2} * beta_{2} + gamma{2} + a_at_z{2}) *
+                  (sigma_1_at_z{2} * beta_{2} + gamma{2} + b_at_z{2}) *
+                  (sigma_2_at_z{2} * beta_{2} + gamma{2} + c_at_z{2}) *
+                  sigma_3{2})
+                ) /\
+              copy_permutation_first_aggregated_commitment_coeff{1} = (                                
+                alpha{2}^4 * (z{2} * beta_{2} + gamma{2} + a_at_z{2}) *                               
+                (z{2} * beta_{2} * k0{2} + gamma{2} + b_at_z{2}) * 
+                (z{2} * beta_{2} * k1{2} + gamma{2} + c_at_z{2}) * 
+                (z{2} * beta_{2} * k2{2} + gamma{2} + d_at_z{2}) + 
+                l_0_at_z{2} * alpha{2}^5
+              ) * v{2} /\
+              lookupSFirstAggregatedCommitment{1} = v{2} * alpha{2}^6 * z_lookup_at_z_omega{2} * (z{2} - omega{2}^(n{2}-1)) /\
+              lookupGrandProductFirstAggregatedCoefficient{1} = ((
+                - alpha{2}^6 * (FieldR.one + beta'{2}) * (gamma'{2} + f_at_z{2}) * (z{2} - omega{2}^(n{2}-1)) * (
+                  gamma'{2}*(FieldR.one + beta'{2}) + t_at_z{2} + beta'{2} * t_at_z_omega{2}
+                )) +
+                alpha{2}^7 * l_0_at_z{2} +
+                alpha{2}^8 * l_n_minus_one_at_z{2}) * v{2} /\
+              query_t_poly_aggregated{1} = t{2} /\
+              d1{2} = main_gate_selector_at_z{2} * (
+                  (a_at_z{2} * q_a{2}) +
+                  (b_at_z{2} * q_b{2}) +
+                  (c_at_z{2} * q_c{2}) +
+                  (d_at_z{2} * q_d{2}) +
+                  (a_at_z{2} * b_at_z{2} * q_ab{2}) +
+                  (a_at_z{2} * c_at_z{2} * q_ac{2}) +
+                  q_const{2} +
+                  (d_at_z_omega{2} * q_d_next{2})
+              ) 
+              + alpha{2} * (
+                (
+                  (a_at_z{2}^2 - b_at_z{2}) +
+                  (b_at_z{2}^2 - c_at_z{2}) * alpha{2} +
+                  (a_at_z{2} * c_at_z{2} - d_at_z{2}) * alpha{2}^2
+                )
+              )* custom_gate_selector{2}
+              + alpha{2}^4 *
+                (a_at_z{2} + beta_{2} * z{2}         + gamma{2}) *                               
+                (b_at_z{2} + beta_{2} * z{2} * k0{2} + gamma{2}) * 
+                (c_at_z{2} + beta_{2} * z{2} * k1{2} + gamma{2}) * 
+                (d_at_z{2} + beta_{2} * z{2} * k2{2} + gamma{2}) * z_perm{2}
+              + G.inv (alpha{2}^4 * z_perm_at_z_omega{2} * beta_{2} *
+                (a_at_z{2} + beta_{2} * sigma_0_at_z{2} + gamma{2}) *
+                (b_at_z{2} + beta_{2} * sigma_1_at_z{2} + gamma{2}) *
+                (c_at_z{2} + beta_{2} * sigma_2_at_z{2} + gamma{2}) *
+                sigma_3{2})
+              + alpha{2}^5 * l_0_at_z{2} * z_perm{2}
+              + G.inv (alpha{2}^6 * (FieldR.one + beta'{2}) * (gamma'{2} + f_at_z{2}) * (z{2} - omega{2}^(n{2}-1)) *
+                (gamma'{2}*(FieldR.one + beta'{2}) + t_at_z{2} + beta'{2} * t_at_z_omega{2}) * z_lookup{2}
+              ) 
+                + alpha{2}^6 * z_lookup_at_z_omega{2} * (z{2} - omega{2}^(n{2}-1)) * s{2}
+                + alpha{2}^7 * l_0_at_z{2} * z_lookup{2}
+                + alpha{2}^8 * l_n_minus_one_at_z{2} * z_lookup{2}  /\
+              f_at_z{2} = lookup_selector_at_z{2} * (a_at_z{2} + eta_{2} * b_at_z{2} + eta_{2}^2 * c_at_z{2} + eta_{2}^3 * table_type_at_z{2})
+            ).
+              progress.
+                exists _copy_permutation_grand_product{1}.
+                exists _copy_permutation_grand_product_opening_at_z_omega{1}.
+                exists _copy_permutation_poly_0_opening_at_z{1}.
+                exists _copy_permutation_poly_1_opening_at_z{1}.
+                exists _copy_permutation_poly_2_opening_at_z{1}.
+                exists _gate_selector_0_opening_at_z{1}.
+                exists _linearisation_poly_opening_at_z{1}.
+                exists _lookup_grand_product{1}.
+                exists _lookup_grand_product_opening_at_z_omega{1}.
+                exists _lookup_s_poly{1}.
+                exists _lookup_s_poly_opening_at_z_omega{1}.
+                exists _lookup_selector_poly_opening_at_z{1}.
+                exists _lookup_t_poly_opening_at_z{1}.
+                exists _lookup_t_poly_opening_at_z_omega{1}.
+                exists _lookup_table_type_poly_opening_at_z{1}.
+                exists _opening_proof_at_z{1}.
+                exists _opening_proof_at_z_omega{1}.
+                exists _public_input{1}.
+                exists _quotient_poly_opening_at_z{1}.
+                exists _quotient_poly_part_0{1}.
+                exists _quotient_poly_part_1{1}.
+                exists _quotient_poly_part_2{1}.
+                exists _quotient_poly_part_3{1}.
+                exists _recursive_part_p1{1}.
+                exists _recursive_part_p2{1}.
+                exists _state_poly_0{1}.
+                exists _state_poly_0_opening_at_z{1}.
+                exists _state_poly_1{1}.
+                exists _state_poly_1_opening_at_z{1}.
+                exists _state_poly_2{1}.
+                exists _state_poly_2_opening_at_z{1}.
+                exists _state_poly_3{1}.
+                exists _state_poly_3_opening_at_z{1}.
+                exists _state_poly_3_opening_at_z_omega{1}.
+                exists alpha2{1}.
+                exists alpha3{1}.
+                exists alpha4{1}.
+                exists alpha5{1}.
+                exists alpha6{1}.
+                exists alpha7{1}.
+                exists alpha8{1}.
+                exists beta_gamma_plus_gamma{1}.
+                exists beta_plus_one{1}.
+                exists failed{1}.
+                exists l0_at_z{1}.
+                exists ln_minus_one_at_z{1}.
+                exists state_alpha{1}.
+                exists state_beta{1}.
+                exists state_beta_lookup{1}.
+                exists state_eta{1}.
+                exists state_gamma{1}.
+                exists state_gamma_lookup{1}.
+                exists state_u{1}.
+                exists state_v{1}.
+                exists state_z{1}.
+                exists state_z_in_domain{1}.
+                exists vk_recursive_flag{1}.
+                exists z_minus_last_omega{1}.
+                by progress; case H; progress.
+                
+                progress. right.
+                  rewrite H H0 H1.
+                  progress.
+                call prepareQueries_high_equiv_super_high. skip. progress.
+                  by rewrite /Constants.DOMAIN_SIZE; trivial.
+             
+                inline PrepareQueries.super_high.
+                wp. skip. progress.
+                rewrite FieldR.ComRing.mulrA. congr.
+                exact FieldR.ComRing.mulrA.
+
+
+(* old proof *)
       seq 5 5: (
         (failed{1} /\ !isValid{2}) \/
         (!failed{1} /\ isValid{2} /\
